Works

OwlLean/OwlLang/Owl.lean
@@ -1,19 +1,22 @@
 import Lean
+import OwlLean.OwlLang.ScopeMap
+
+open ScopeMap
 
 namespace Owl
 
 
-structure Lattice where
-  labels : Type
-  leq    : labels -> labels -> Prop
-  bot    : labels
-  bot_proof : forall (l : labels), (leq bot l) = true
-  join   : labels -> labels -> labels
-  meet   : labels -> labels -> labels
-  leq_trans : forall l1 l2 l3, leq l1 l2 -> leq l2 l3 -> leq l1 l3
-  leq_refl : forall l, leq l l
-  bot_all : forall l, leq bot l
-  join_le : forall l1 l2 l3, leq l1 l3 -> leq l2 l3 -> leq (join l1 l2) l3
+-- structure Lattice where
+--   labels : Type
+--   leq    : labels -> labels -> Prop
+--   bot    : labels
+--   bot_proof : forall (l : labels), (leq bot l) = true
+--   join   : labels -> labels -> labels
+--   meet   : labels -> labels -> labels
+--   leq_trans : forall l1 l2 l3, leq l1 l2 -> leq l2 l3 -> leq l1 l3
+--   leq_refl : forall l, leq l l
+--   bot_all : forall l, leq bot l
+--   join_le : forall l1 l2 l3, leq l1 l3 -> leq l2 l3 -> leq (join l1 l2) l3
 
 inductive LabelTm where
   | atom : String -> LabelTm
@@ -22,6 +25,7 @@ inductive LabelTm where
   | bot : LabelTm
   deriving BEq, Repr, Lean.ToExpr
 
+@[simp]
 def LabelTm.interp (t : LabelTm) (p : String -> Bool) : Bool :=
   match t with
   | .atom x => p x
@@ -33,77 +37,58 @@ def LabelTm.interp (t : LabelTm) (p : String -> Bool) : Bool :=
 def LabelTm.leq (l1 : LabelTm) (l2 : LabelTm) :=
   forall p, (! l2.interp p) || l1.interp p
 
-def L : Lattice := {
-    labels := LabelTm,
-    leq := LabelTm.leq,
-    bot := .bot,
-    bot_proof := by
-      intros l
-      simp [LabelTm.leq]
-      simp [LabelTm.interp]
-    join := .and,
-    meet := .or,
-    leq_trans := by
-      intros l1 l2 l3
-      unfold LabelTm.leq
-      intros h1 h2 p
-      grind
-    leq_refl := by
-      unfold LabelTm.leq
-      grind
-    bot_all := by
-      unfold LabelTm.leq
-      simp [LabelTm.interp]
-    join_le := by
-      intros l1 l2 l3 h1 h2
-      simp [LabelTm.leq, LabelTm.interp] at *
-      intros
-      grind
-}
+-- def labelTmLattice : Lattice := {
+--     labels := LabelTm,
+--     leq := LabelTm.leq,
+--     bot := .bot,
+--     bot_proof := by
+--       intros l
+--       simp [LabelTm.leq]
+--       simp [LabelTm.interp]
+--     join := .and,
+--     meet := .or,
+--     leq_trans := by
+--       intros l1 l2 l3
+--       unfold LabelTm.leq
+--       intros h1 h2 p
+--       grind
+--     leq_refl := by
+--       unfold LabelTm.leq
+--       grind
+--     bot_all := by
+--       unfold LabelTm.leq
+--       simp [LabelTm.interp]
+--     join_le := by
+--       intros l1 l2 l3 h1 h2
+--       simp [LabelTm.leq, LabelTm.interp] at *
+--       intros
+--       grind
+-- }
 
 
-instance : Lean.ToExpr L.labels := by
-  unfold L
-  simp
-  infer_instance
 
-instance : Repr L.labels := by
-  unfold L
-  simp
-  infer_instance
+def lattice_leq_trans : forall {l1 l2 l3}, LabelTm.leq l1 l2 -> LabelTm.leq l2 l3 -> LabelTm.leq l1 l3 :=
+  fun {l1 l2 l3} => by
+     intros
+     grind [LabelTm.leq]
 
-def lattice_leq_trans : forall {l1 l2 l3}, L.leq l1 l2 -> L.leq l2 l3 -> L.leq l1 l3 :=
-  fun {l1 l2 l3} =>
-    L.leq_trans l1 l2 l3
 
-grind_pattern lattice_leq_trans => L.leq l1 l2, L.leq l2 l3
+grind_pattern lattice_leq_trans => LabelTm.leq l1 l2, LabelTm.leq l2 l3
 
-def lattice_leq_refl : forall {l}, L.leq l l := fun {l} => L.leq_refl l
+def lattice_leq_refl : forall {l}, LabelTm.leq l l := fun {l} => by
+  grind [LabelTm.leq]
 
-grind_pattern lattice_leq_refl => L.leq l l
+def lattice_bot_all : forall {l}, LabelTm.leq LabelTm.bot l := fun {l} => by
+  simp [LabelTm.leq]
 
-def lattice_bot_all : forall {l}, L.leq L.bot l := fun {l} => L.bot_all l
+grind_pattern lattice_bot_all => LabelTm.leq LabelTm.bot l
 
-grind_pattern lattice_bot_all => L.leq L.bot l
-
-def lattice_join_bot : forall {l}, L.leq (L.join L.bot l) l := by
+def lattice_join_bot : forall {l}, LabelTm.leq (LabelTm.and LabelTm.bot l) l := by
   intros
-  apply L.join_le
-  grind
-  grind
+  simp [LabelTm.leq]
 
-grind_pattern lattice_join_bot => (L.join L.bot l)
+grind_pattern lattice_join_bot => (LabelTm.and LabelTm.bot l)
 
-@[simp]
-theorem leq_bot : L.leq L.bot l := by
-  grind
-
-abbrev Lcarrier : Type := L.labels
-
-instance : BEq Lcarrier := by
-  unfold Lcarrier
-  simp [L]
-  infer_instance
 
 
 structure opaqueSyntax where
@@ -112,87 +97,7 @@ structure opaqueSyntax where
 instance : Repr opaqueSyntax where
   reprPrec _ _ := f!"<syntax>"
 
-structure Scope where
-  nLbl : Nat
-  nRef : Nat
-  nTy : Nat
-  nTm : Nat
-  deriving BEq, Lean.ToExpr
-
-abbrev Scope.empty : Scope := {
-  nLbl := 0
-  nRef := 0
-  nTy := 0
-  nTm := 0
-}
-
-abbrev Scope.withoutTms (s : Scope) : Scope := { s with nTm := 0 }
-
-class Scope.closedTm (s : Scope) where
-  h : s.nTm = 0
-
-
-abbrev Scope.bumpRef (s : Scope) := { s with nRef := s.nRef + 1 }
-abbrev Scope.bumpTy (s : Scope) := { s with nTy := s.nTy + 1 }
-abbrev Scope.bumpLbl (s : Scope) := { s with nLbl := s.nLbl + 1 }
-abbrev Scope.bumpTm (s : Scope) := { s with nTm := s.nTm + 1 }
-
-structure Scope.renaming (s s' : Scope) where
-  renameLbl : Fin s.nLbl -> Fin s'.nLbl
-  renameRef : Fin s.nRef -> Fin s'.nRef
-  renameTy : Fin s.nTy -> Fin s'.nTy
-  renameTm : Fin s.nTm -> Fin s'.nTm
-
-def up_ren (xi : Fin m -> Fin n) : Fin (m + 1) -> Fin (n + 1) :=
-  Fin.cases 0 (Fin.succ ∘ xi)
-
-abbrev Scope.renaming.bumpRef {s : Scope} (r : s.renaming s') : s.bumpRef.renaming s'.bumpRef := {
-  r with
-    renameRef := up_ren r.renameRef
-}
-
-abbrev Scope.renaming.bumpTy {s : Scope} (r : s.renaming s') : s.bumpTy.renaming s'.bumpTy := {
-  r with
-    renameTy := up_ren r.renameTy
-}
-
-abbrev Scope.renaming.bumpLbl {s : Scope} (r : s.renaming s') : s.bumpLbl.renaming s'.bumpLbl := {
-  r with
-    renameLbl := up_ren r.renameLbl
-}
-
-abbrev Scope.renaming.bumpTm {s : Scope} (r : s.renaming s') : s.bumpTm.renaming s'.bumpTm := {
-  r with
-    renameTm := up_ren r.renameTm
-}
-
-abbrev Scope.liftRef {s : Scope} : s.renaming s.bumpRef := {
-  renameLbl := id
-  renameTy := id
-  renameRef := Fin.succ
-  renameTm := id
-}
-
-abbrev Scope.liftTy {s : Scope} : s.renaming s.bumpTy := {
-  renameLbl := id
-  renameTy := Fin.succ
-  renameRef := id
-  renameTm := id
-}
-
-abbrev Scope.liftLbl {s : Scope} : s.renaming s.bumpLbl := {
-  renameLbl := Fin.succ
-  renameTy := id
-  renameRef := id
-  renameTm := id
-}
-
-abbrev Scope.liftTm {s : Scope} : s.renaming s.bumpTm := {
-  renameLbl := id
-  renameTy := id
-  renameRef := id
-  renameTm := Fin.succ
-}
+open Lean
 
 inductive cond_sym : Type
 | leq : cond_sym
@@ -205,30 +110,36 @@ inductive cond_sym : Type
 | nlt : cond_sym
 deriving Repr, DecidableEq, Lean.ToExpr
 
+syntax (name := L) "L" : term
+macro_rules
+  | `(L) => `(0)
 
-inductive label : Scope -> Type where
-| var_label : String -> Fin s.nLbl -> label s
-| latl : Lcarrier -> label s
+syntax (name := R) "R" : term
+macro_rules
+  | `(R) => `(1)
+
+syntax (name := Ty) "Ty" : term
+macro_rules
+  | `(Ty) => `(2)
+
+syntax (name := Tm) "Tm" : term
+macro_rules
+  | `(Tm) => `(3)
+
+inductive label : ScopeMap 1 -> Type where
+| var_label : String -> Fin (s.get 0) -> label s
+| latl : LabelTm -> label s
 | ljoin : label s -> label s -> label s
 | lmeet : label s -> label s -> label s
-| default : label s
 deriving Repr, BEq, Lean.ToExpr
 
-def label.downRef {s:Scope} (l : label s.bumpRef) : label s :=
-  match l with
-  | .var_label s0 i => .var_label s0 i
-  | .latl x => .latl x
-  | .ljoin l1 l2 => .ljoin (l1.downRef) (l2.downRef)
-  | .lmeet l1 l2 => .lmeet (l1.downRef) (l2.downRef)
-  | .default => .default
 
-
-inductive corruption : Scope -> Type where
+inductive corruption : ScopeMap 1 -> Type where
 | corr : label s -> corruption s
 | not_corr : label s -> corruption s
 deriving Repr, BEq, Lean.ToExpr
 
-inductive constr  : Scope -> Type where
+inductive constr  : ScopeMap 1 -> Type where
 | condition : cond_sym -> label s -> label s -> constr s
 deriving Repr, BEq, Lean.ToExpr
 
@@ -242,47 +153,47 @@ deriving instance BEq, Lean.ToExpr for Lean.Syntax
 deriving instance BEq, Lean.ToExpr for Owl.opaqueSyntax
 
 
-inductive rexp : Scope -> Type where
+-- TODO: remove tmvar, get ScopeMap 2; simplifiy the implementation
+inductive rexp : ScopeMap 2 -> Type where
   | fvar : Lean.Name -> rexp s
-  | var : Fin s.nRef -> rexp s
+  | var : Fin (s.get R) -> rexp s
   | op : String -> rexp s -> rexp s -> rexp s
-  | tmvar : Fin s.nTm -> rexp s
   | const : String -> rexp s
 deriving Repr, BEq, Lean.ToExpr
 
 
 
-inductive prop : Scope -> Type where
+inductive prop : ScopeMap 2 -> Type where
   | peq : rexp s -> rexp s -> prop s
   | pand : prop s -> prop s -> prop s
   | por : prop s -> prop s -> prop s
   | pimpl : prop s -> prop s -> prop s
   | pnot : prop s -> prop s
-  | pall : prop s.bumpRef -> prop s
+  | pall : prop (s.bump R) -> prop s
   deriving Repr, BEq, Lean.ToExpr
 
 
 
 
-inductive ty : Scope -> Type where
-| var_ty : Fin s.nTy -> ty s
+inductive ty : ScopeMap 3 -> Type where
+| var_ty : Fin (s.get Ty) -> ty s
 | Any : ty s
 | Unit : ty s
-| RData : label s -> rexp s -> ty s
-| Data : label s -> ty s
+| RData : label (s.restrict 1) -> rexp (s.restrict 2) -> ty s
+| Data : label (s.restrict 1) -> ty s
 | Ref : ty s -> ty s
 | arr : ty s -> ty s -> ty s
 | union : ty s -> ty s -> ty s
 | inter : ty s -> ty s -> ty s
 | prod : ty s -> ty s -> ty s
 | sum : ty s -> ty s -> ty s
-| all : ty s -> ty s.bumpTy -> ty s
-| ex : ty s -> ty s.bumpTy -> ty s
-| ex_r : ty s.bumpRef -> ty s
-| all_r : ty s.bumpRef -> ty s
-| all_l : cond_sym -> label s -> ty s.bumpLbl -> ty s
-| t_if : label s -> ty s -> ty s -> ty s
-| refined : ty s -> prop s -> ty s
+| all : ty s -> ty (s.bump Ty) -> ty s
+| ex : ty s -> ty (s.bump Ty) -> ty s
+| ex_r : ty (s.bump R) -> ty s
+| all_r : ty (s.bump R) -> ty s
+| all_l : cond_sym -> label (s.restrict 1) -> ty (s.bump L) -> ty s
+| t_if : label (s.restrict 1) -> ty s -> ty s -> ty s
+| refined : ty s -> prop (s.restrict 2) -> ty s
 | Public : ty s
 | default : ty s
 | admit : ty s
@@ -292,23 +203,23 @@ deriving Repr, BEq, Lean.ToExpr
 
 mutual
 
-  inductive tm : Scope -> Type where
+  inductive tm : ScopeMap 4 -> Type where
    | mk : opaqueSyntax -> tmX s -> tm s
    deriving Repr, Lean.ToExpr
 
-inductive tmX : Scope -> Type where
+inductive tmX : ScopeMap 4 -> Type where
 | admit : tmX s
-| var_tm : Fin s.nTm -> tmX s
+| var_tm : Fin (s.get Tm) -> tmX s
 | error : tmX s
 | skip : tmX s
 | bitstring : String -> tmX s
 | loc : Nat -> tmX s
-| fixlam : String -> tm (s.bumpTm.bumpTm) -> tmX s
-| tlet : tm s -> tm s.bumpTm -> tmX s
-| union_elim : tm s -> tm s.bumpTm -> tmX s
-| tlam : tm s.bumpTy -> tmX s
-| rlam : tm s.bumpRef -> tmX s
-| l_lam : tm s.bumpLbl -> tmX s
+| fixlam : String -> tm ((s.bump Tm).bump Tm) -> tmX s
+| tlet : tm s -> tm (s.bump Tm) -> tmX s
+| union_elim : tm s -> tm (s.bump Tm) -> tmX s
+| tlam : tm (s.bump Ty) -> tmX s
+| rlam : tm (s.bump R) -> tmX s
+| l_lam : tm (s.bump L) -> tmX s
 | Op : String -> tm s -> tm s -> tmX s
 | zero : tm s -> tmX s
 | app : tm s -> tm s -> tmX s
@@ -322,54 +233,203 @@ inductive tmX : Scope -> Type where
 | inr  : tm s -> tmX s
 | case :
     tm s ->
-    tm s.bumpTm -> tm s.bumpTm -> tmX s
-| tapp : tm s -> ty s -> tmX s
-| lapp : tm s -> label s -> tmX s
-| rapp : tm s -> rexp s -> tmX s
-| pack : ty s -> tm s -> tmX s
-| rpack : rexp s -> tm s -> tmX s
-| unpack : tm s -> tm s.bumpTy.bumpTm -> tmX s
+    tm (s.bump Tm) -> tm (s.bump Tm) -> tmX s
+| tapp : tm s -> ty (s.restrict 3) -> tmX s
+| lapp : tm s -> label (s.restrict 1) -> tmX s
+| rapp : tm s -> rexp (s.restrict 2) -> tmX s
+| pack : ty (s.restrict 3) -> tm s -> tmX s
+| rpack : rexp (s.restrict 2) -> tm s -> tmX s
+| unpack : tm s -> tm ((s.bump Ty).bump Tm) -> tmX s
 | if_tm :
     tm s ->
     tm s -> tm s -> tmX s
 | if_c :
-    label s -> tm s -> tm s -> tmX s
+    label (s.restrict 1) -> tm s -> tm s -> tmX s
 | sync : tm s -> tmX s
-| corr_case : label s -> tm s -> tmX s
-| annot : tm s -> ty s -> tmX s
+| corr_case : label (s.restrict 1) -> tm s -> tmX s
+| annot : tm s -> ty (s.restrict 3) -> tmX s
 | default : tmX s
 deriving Repr, Lean.ToExpr
 
 end
 
-def rexp.free (i : Fin s.nRef) (re : rexp s) :=
+def rexp.free (i : Fin (s.get R)) (re : rexp s) :=
   match re with
   | .fvar _ => true
   | .var j      => i != j
   | .op _ r1 r2 => rexp.free i r1 && rexp.free i r2
   | .const _    => true
-  | .tmvar _ => true
+
+
+-- class EqScopeMap (s : ScopeMap N) (t : ScopeMap N) where
+--   heq : s = t
+--
+-- class IsTrue (p : Prop) where
+--   pf : p
+--
+--
+--
+-- class FinToNat (i : Fin n) (m : outParam Nat) where
+--   heq : i.val = m
+--
+-- instance {x : Fin n}: FinToNat x x.val where
+--   heq := rfl
+--
+-- class LeNat (n : Nat) (m : Nat) where
+--   le : n ≤ m
+--
+-- instance : LeNat 0 0 where
+--   le := by simp
+--
+-- instance [h : LeNat n m] : LeNat n (m + 1) where
+--   le := by grind [h.le]
+--
+-- instance [h : LeNat n m] : LeNat (n + 1) (m + 1) where
+--   le := by grind [h.le]
+--
+-- instance {m1 m2 : ScopeMap 2} {p : prop m1} [h : EqScopeMap m1 m2] : CoeDep (prop m1) p (prop m2) where
+--   coe := h.heq ▸ p
+--
+-- instance [h : IsTrue (n =  m)] {i : Fin n} : CoeDep (Fin n) i (Fin m) where
+--   coe := i.cast h.pf
+--
+-- instance [h : IsTrue (m = n)] {i : Fin n} : CoeDep (Fin n) i (Fin m) where
+--   coe := i.cast h.pf.symm
+--
+-- class SameFin (i : Fin n) (j : Fin m) where
+--   same : i.val = j.val
+--
+-- class NeqFin (i : Fin n) (j : Fin m) where
+--   h : ¬ i.val = j.val
+--
+-- class GeFinNat (i : Fin n) (j : Nat) where
+--   h : i.val >= j
+--
+--
+-- instance {s : ScopeMap N} {i : Fin N} {M : Nat} {h h' : M ≤ N} [hiM : GeFinNat i M] : EqScopeMap ((s.bump i).restrict M h) (s.restrict M h') where
+--   heq := by
+--     simp [ScopeMap.bump_restrict]
+--     intros
+--     cases hiM
+--     grind
+--
+--
+-- instance [h : NeqFin x y] : NeqFin y x where
+--   h := by cases h; grind
+--
+--
+--
+-- instance [h : SameFin x y] : SameFin y x where
+--   same := h.same.symm
+--
+-- instance : SameFin (1 : Fin 4) (1 : Fin 3) where
+--   same := by simp
+--
+-- instance {s : ScopeMap N} {M : Nat} {hM} {x : Fin M} {y} [hxy : SameFin x y] : IsTrue ((s.restrict M hM).get x = s.get y) where
+--   pf := by
+--     simp
+--     unfold ScopeMap.get
+--     congr 1
+--     apply Fin.ext
+--     simp
+--     apply hxy.same
+--
+-- instance {s : ScopeMap N} {M : Nat} {hM : M <= N} {M' : Nat} {hM' : M' <= M} {h3 : M' <= N} :
+--    EqScopeMap ((s.restrict M hM).restrict M' hM') ((s.restrict M' h3))  where
+--      heq := by
+--       apply ScopeMap.restrict_restrict
+--
+--
+--
+--
+-- instance {s : ScopeMap N} {x y : Fin N} [h : NeqFin x y] : IsTrue ((s.bump x).get y = s.get y) where
+--   pf := by cases h; simp; grind
+--
+-- instance : NeqFin (1 : Fin 4) (3 : Fin 4) where
+--   h := by grind
+--
+-- instance : NeqFin (0 : Fin 4) (1 : Fin 4) where
+--   h := by grind
+--
+-- instance {s : ScopeMap N} {x : Fin N} : IsTrue ((s.bump x).get x = s.get x + 1) where
+--   pf := by simp
+--
+-- instance {s : ScopeMap N} {x : Fin N} : IsTrue (s.get x + 1 = (s.bump x).get x) where
+--   pf := by simp
+--
+-- instance : SameFin (2 : Fin 3) (2 : Fin 4) where
+--   same := by simp
+--
+-- instance {s : ScopeMap N} (x : Fin N) M h (y : Fin M) [Hsame : SameFin x y] : EqScopeMap ((s.bump x).restrict M h) ((s.restrict M h).bump y) where
+--   heq := by
+--      simp [ScopeMap.bump_restrict]
+--      split
+--      congr 1
+--      cases Hsame; grind
+--      cases y
+--      cases x
+--      cases Hsame
+--      grind
+--
+--
+-- instance : GeFinNat (2 : Fin 4) 1 where
+--   h := by simp
+--
+-- instance [h : EqScopeMap s t] (l : label s) : CoeDep (label s) l (label t) where
+--   coe := h.heq ▸ l
+--
+-- instance [h : EqScopeMap s t] (l : ty s) : CoeDep (ty s) l (ty t) where
+--   coe := h.heq ▸ l
+--
+-- instance [h : EqScopeMap s t] (p : prop s) : CoeDep (prop s) p (prop t) where
+--   coe := h.heq ▸ p
+--
+-- instance {s : ScopeMap N} : EqScopeMap ((s.bump x).bump y) ((s.bump y).bump x) where
+--    heq := by simp [ScopeMap.bump_bump]
+--
+-- instance {s : ScopeMap N} {x : Fin N} {M : Nat} {h : M <= N} {y : Fin M} [heq : SameFin x y] :  EqScopeMap ((s.bump x).restrict M h) ((s.restrict M h).bump y) where
+--   heq := by
+--     simp [ScopeMap.bump_restrict]
+--     split
+--     congr 1
+--     cases heq
+--     grind
+--     cases y
+--     cases heq
+--     grind
+--
+-- instance {s : ScopeMap N} {x : Fin N} {M : Nat} {h h' : M <= N} [h2 : IsTrue (x >= M)] :  EqScopeMap ((s.bump x).restrict M h) (s.restrict M h') where
+--   heq := by
+--     simp [ScopeMap.bump_restrict]
+--     intros
+--     cases h2
+--     grind
+
+#eval (1 : Fin 3)
+
+#check OfNat
+
 
 @[simp]
-def prop.rfree  (p : prop s) (i : Fin s.nRef) : Bool :=
+def prop.rfree  (p : prop s) (i : Fin (s.get R)) : Bool :=
   match p with
   | .peq re1 re2 => rexp.free i re1 && rexp.free i re2
   | .pand p1 p2 => prop.rfree p1 i && prop.rfree p2 i
   | .por p1 p2 => prop.rfree p1 i && prop.rfree p2 i
   | .pimpl p1 p2 => prop.rfree p1 i && prop.rfree p2 i
   | .pnot p1 => prop.rfree p1 i
-  | .pall p0 => prop.rfree p0 (Fin.succ i)
+  | .pall p0 => prop.rfree p0 ((Fin.succ i).cast (by simp))
 
 
 @[simp]
-def ty.r_free (t : ty s) (i : Fin s.nRef) : Bool :=
+def ty.r_free (t : ty s) (i : Fin (s.get R)) : Bool :=
   match t with
 | .admit => true
 | .var_ty _ => true
 | .Any => true
-| .refined t0 p => t0.r_free i && p.rfree i
+| .refined t0 p => t0.r_free i && p.rfree (i.cast (by simp))
 | .Unit => true
-| .RData _ re => rexp.free i re
+| .RData _ re => rexp.free (i.cast (by simp)) re
 | .Data _ => true
 | .Ref t => t.r_free i
 | .arr t1 t2 => t1.r_free i && t2.r_free i
@@ -377,11 +437,11 @@ def ty.r_free (t : ty s) (i : Fin s.nRef) : Bool :=
 | .inter t1 t2 => t1.r_free i && t2.r_free i
 | .prod t1 t2 => t1.r_free i && t2.r_free i
 | .sum t1 t2 => t1.r_free i && t2.r_free i
-| .all t1 t2 => t1.r_free i && t2.r_free i
-| .ex t1 t2 => t1.r_free i && t2.r_free i
-| .ex_r t0 => t0.r_free (Fin.succ i)
-| .all_r t0 => t0.r_free (Fin.succ i)
-| .all_l _ _ t => t.r_free i
+| .all t1 t2 => t1.r_free i && t2.r_free (i.cast (by simp))
+| .ex t1 t2 => t1.r_free i && t2.r_free (i.cast (by simp))
+| .ex_r t0 => t0.r_free ((Fin.succ i).cast (by simp))
+| .all_r t0 => t0.r_free ((Fin.succ i).cast (by simp))
+| .all_l _ _ t => t.r_free (i.cast (by simp))
 | .t_if _ t1 t2 => t1.r_free i && t2.r_free i
 | .Public => true
 | .default => true
@@ -442,11 +502,10 @@ def label.rename
   (l : label s) (ren : s.renaming s')
   : label s' :=
   match l with
-  | .var_label n s0 => label.var_label n (ren.renameLbl s0)
+  | .var_label n s0 => label.var_label n (ren.apply L s0)
   | .latl s0 => label.latl s0
   | .ljoin s0 s1 => label.ljoin (s0.rename ren) (s1.rename ren)
   | .lmeet s0 s1 => label.lmeet (s0.rename ren) (s1.rename ren)
-  | .default => .default
 
 def constr.rename
   (c : constr s)
@@ -465,11 +524,10 @@ def corruption.rename
 def rexp.rename (r : rexp s) (ren : s.renaming s')
   : rexp s' :=
     match r with
-    | .fvar i => .fvar i
-    | .var j => .var (ren.renameRef j)
+    | .fvar nm => .fvar nm
+    | .var j => .var (ren.apply R j)
     | .op s r1 r2 => .op s (r1.rename ren) (r2.rename ren)
     | .const b => .const b
-    | .tmvar j => .tmvar (ren.renameTm j)
 
 def prop.rename (p : prop s) (ren : s.renaming s') : prop s' :=
   match p with
@@ -478,18 +536,18 @@ def prop.rename (p : prop s) (ren : s.renaming s') : prop s' :=
   | .por p1 p2 => .por (p1.rename ren) (p2.rename ren)
   | .pimpl p1 p2 => .pimpl (p1.rename ren) (p2.rename ren)
   | .pnot p1 => .pnot (p1.rename ren)
-  | .pall p => .pall (p.rename ren.bumpRef)
+  | .pall p => .pall (p.rename (ren.bump R))
 
 
 @[simp]
 def ty.rename (t : ty s) (ren : s.renaming s') : ty s' :=
   match t with
   | .admit => .admit
-  | .var_ty s0 => .var_ty (ren.renameTy s0)
+  | .var_ty s0 => .var_ty (ren.apply Ty s0)
   | .Any => .Any
   | .Unit => .Unit
-  | .RData s0 re => .RData (s0.rename ren) (re.rename ren)
-  | .Data s0 => .Data (s0.rename ren)
+  | .RData s0 re => .RData (s0.rename $ ren.restrict) (re.rename $ ren.restrict)
+  | .Data s0 => .Data (s0.rename $ ren.restrict)
   | .Ref s0 => .Ref (s0.rename ren)
   | .arr s0 s1 =>
       .arr (s0.rename ren) (s1.rename ren)
@@ -500,22 +558,22 @@ def ty.rename (t : ty s) (ren : s.renaming s') : ty s' :=
   | .prod s0 s1 =>
       .prod (s0.rename ren) (s1.rename ren)
   | .refined t p =>
-      .refined (t.rename ren) (p.rename ren)
+      .refined (t.rename ren) (p.rename $ ren.restrict)
   | .sum s0 s1 =>
       .sum (s0.rename ren) (s1.rename ren)
   | .all s0 s1 =>
       .all (s0.rename ren)
-           (s1.rename ren.bumpTy)
+           (s1.rename $ ren.bump Ty)
   | .ex s0 s1 =>
       .ex (s0.rename ren)
-           (s1.rename ren.bumpTy)
-  | .ex_r t0 => .ex_r (t0.rename ren.bumpRef)
-  | .all_r t0 => .all_r (t0.rename ren.bumpRef)
+           (s1.rename $ ren.bump Ty)
+  | .ex_r t0 => .ex_r (t0.rename $ ren.bump R)
+  | .all_r t0 => .all_r (t0.rename $ ren.bump R)
   | .all_l s0 s1 s2 =>
-      .all_l s0 (s1.rename ren)
-        (s2.rename ren.bumpLbl)
+      .all_l s0 (s1.rename $ ren.restrict _)
+        (s2.rename $ ren.bump L)
   | .t_if s0 s1 s2 =>
-      .t_if (s0.rename ren) (s1.rename ren)
+      .t_if (s0.rename $ ren.restrict _) (s1.rename ren)
         (s2.rename ren)
   | .Public => .Public
   | .default => .default
@@ -534,28 +592,28 @@ def tm.rename
 def tmX.rename (t : tmX s) (ren : s.renaming s') : tmX s' :=
   match t with
   | .admit => .admit
-  | .var_tm s0 => .var_tm (ren.renameTm s0)
+  | .var_tm s0 => .var_tm (ren.apply Tm s0)
   | .error => .error
   | .skip => .skip
   | .bitstring s0 => .bitstring s0
   | .loc s0 => .loc s0
   | .fixlam nm s0 =>
       .fixlam nm
-        (s0.rename ren.bumpTm.bumpTm)
+        (s0.rename $ (ren.bump Tm).bump Tm)
   | .tlam s0 =>
-      .tlam (s0.rename ren.bumpTy)
+      .tlam (s0.rename $ ren.bump Ty)
   | .rlam s0 =>
     .rlam
-        (s0.rename ren.bumpRef)
+        (s0.rename $ ren.bump R)
   | .tlet e1 e2 =>
     .tlet (e1.rename ren)
-          (e2.rename ren.bumpTm)
+          (e2.rename $ ren.bump Tm)
   | .union_elim e1 e2 =>
     .union_elim (e1.rename ren)
-                (e2.rename ren.bumpTm)
+                (e2.rename $ ren.bump Tm)
   | .l_lam s0 =>
       .l_lam
-        (s0.rename ren.bumpLbl)
+        (s0.rename $ ren.bump L)
   | .Op s0 s1 s2 =>
       .Op s0 (s1.rename ren)
         (s2.rename ren)
@@ -581,87 +639,87 @@ def tmX.rename (t : tmX s) (ren : s.renaming s') : tmX s' :=
   | .inr s0 => .inr (s0.rename ren)
   | .case s0 s1 s2 =>
       .case (s0.rename ren)
-            (s1.rename ren.bumpTm)
-            (s2.rename ren.bumpTm)
+            (s1.rename $ ren.bump Tm)
+            (s2.rename $ ren.bump Tm)
   | .tapp s0 s1 =>
       .tapp (s0.rename ren)
-        (s1.rename ren)
+        (s1.rename $ ren.restrict)
   | .lapp s0 s1 =>
       .lapp (s0.rename ren)
-            (s1.rename ren)
+            (s1.rename $ ren.restrict)
   | .rapp e0 re =>
       .rapp (e0.rename ren)
-            (re.rename ren)
+            (re.rename $ ren.restrict)
   | .pack s s0 => .pack
-    (s.rename ren)
+    (s.rename $ ren.restrict)
     (s0.rename ren)
-  | .rpack re t0 => .rpack (re.rename ren) (t0.rename ren)
+  | .rpack re t0 => .rpack (re.rename $ ren.restrict) (t0.rename ren)
   | .unpack s0 s1 =>
       .unpack (s0.rename ren)
-              (s1.rename ren.bumpTy.bumpTm)
+              (s1.rename $ (ren.bump Ty).bump Tm)
   | .if_tm s0 s1 s2 =>
       .if_tm (s0.rename ren)
              (s1.rename ren) (s2.rename ren)
   | .if_c s0 s1 s2 =>
-      .if_c (s0.rename ren)
+      .if_c (s0.rename $ ren.restrict)
             (s1.rename ren)
             (s2.rename ren)
   | .sync s0 => .sync (s0.rename ren)
-  | .corr_case lab e => .corr_case (lab.rename ren) (e.rename ren)
-  | .annot e t => .annot (e.rename ren) (t.rename ren)
+  | .corr_case lab e => .corr_case (lab.rename $ ren.restrict) (e.rename ren)
+  | .annot e t => .annot (e.rename ren) (t.rename $ ren.restrict)
   | .default => .default
 end
 
+abbrev OwlFunctors (x : Fin 3) : ScopeFunctor 3 x :=
+  match x with
+  | ⟨L, _⟩ => ⟨fun m => label (m.restrict 1), fun m m' r x => x.rename (r.restrict) , fun i => .var_label "_" (by simpa using i)⟩
+  | ⟨R, _⟩  => ⟨fun m => rexp (m.restrict _), fun m m' r x => x.rename (r.restrict) , fun i => .var (by simpa using i)⟩
+  | ⟨Ty, _⟩ => ⟨fun m => ty m, fun m m' r x => x.rename r, fun i => .var_ty (by simpa using i)⟩
+--  | ⟨Tm, _⟩ => ⟨fun m => Fin (m.get _), fun m m' r i => r.apply _ i, fun i => i⟩
 
-structure Scope.subst (s s' : Scope) where
-  substLbl : Fin s.nLbl -> label s'
-  substRef : Fin s.nRef -> rexp s'
-  substTy : Fin s.nTy -> ty s'
-  substTm : Fin s.nTm -> rexp s'
+
+abbrev Subst := ScopeMap.Subst 3 OwlFunctors
+
+abbrev LabelFunctors (x : Fin 1) : ScopeFunctor 1 x :=
+  match x with
+  | ⟨0, _⟩  => ⟨fun m => label m, fun m m' r x => x.rename r , fun i => .var_label "_" (by simpa using i)⟩
+
+@[simp]
+abbrev LabelSubst := ScopeMap.Subst 1 LabelFunctors
 
 abbrev mapM [Monad m] (c : m a) (f : a -> b) : m b :=
   c >>= fun x => pure (f x)
 
-abbrev Scope.subst.bumpRef {s : Scope} (sub : s.subst s') : s.bumpRef.subst s'.bumpRef := {
-  substLbl := fun i => (sub.substLbl i).rename Scope.liftRef,
-  substRef := fun i => Fin.cases (.var 0) (fun j => (sub.substRef j).rename Scope.liftRef) i,
-  substTy := fun i => (sub.substTy i).rename Scope.liftRef,
-  substTm := fun i => (sub.substTm i).rename Scope.liftRef
-}
+abbrev RexpFunctors (x : Fin 2) : ScopeFunctor 2 x :=
+  match x with
+  | ⟨L, _⟩  => ⟨fun m => label (m.restrict 1), fun m m' r x => x.rename (r.restrict) , fun i => .var_label "_" (by simpa using i)⟩
+  | ⟨R, _⟩  => ⟨fun m => rexp m, fun m m' r x => x.rename r, fun i => .var (by simpa using i)⟩
+--  | ⟨Tm, _⟩  => ⟨fun m => Fin (m.get _), fun m m' r i => r.apply _ i, fun i => i⟩
 
-abbrev Scope.subst.downRef {s : Scope} (r : rexp s) : s.bumpRef.subst s := {
-  substLbl := fun i => .var_label "_" i,
-  substRef := fun i => Fin.cases r (fun j => .var j) i,
-  substTy := fun i => .var_ty i,
-  substTm := fun i => .tmvar i
-}
+abbrev RexpSubst := ScopeMap.Subst 2 RexpFunctors
 
-abbrev Scope.subst.bumpTy {s : Scope} (sub : s.subst s') : s.bumpTy.subst s'.bumpTy := {
-  substLbl := fun i => (sub.substLbl i).rename Scope.liftTy,
-  substRef := fun i => (sub.substRef i).rename Scope.liftTy,
-  substTy := fun i => Fin.cases (.var_ty 0) (fun j => (sub.substTy j).rename Scope.liftTy) i,
-  substTm := fun i => (sub.substTm i).rename Scope.liftTy
-}
+def Subst.toLabelSubst (sub : Subst s s') : LabelSubst (s.restrict 1) (s'.restrict 1) :=
+  ⟨fun x i =>
+    match x with
+    | 0 => by
+        simp
+        exact (sub.apply 0 (by simpa using i))
+  ⟩
 
-abbrev Scope.subst.bumpLbl {s : Scope} (sub : s.subst s') : s.bumpLbl.subst s'.bumpLbl := {
-  substLbl := fun i => Fin.cases (.var_label "_" 0) (fun j => (sub.substLbl j).rename Scope.liftLbl) i,
-  substRef := fun i => (sub.substRef i).rename Scope.liftLbl,
-  substTy := fun i => (sub.substTy i).rename Scope.liftLbl,
-  substTm := fun i => (sub.substTm i).rename Scope.liftLbl
-}
-
-abbrev Scope.subst.bumpTm {s : Scope} (sub : s.subst s') : s.bumpTm.subst s'.bumpTm := {
-  substLbl := fun i => (sub.substLbl i).rename Scope.liftTm,
-  substRef := fun i => (sub.substRef i).rename Scope.liftTm,
-  substTy := fun i => (sub.substTy i).rename Scope.liftTm,
-  substTm := fun i => Fin.cases (.tmvar 0) (fun j => (sub.substTm j).rename Scope.liftTm) i
-}
+def Subst.toRexpSubst (sub : Subst s s') : RexpSubst (s.restrict 2) (s'.restrict 2) :=
+  ⟨fun x i => by
+    unfold RexpFunctors
+    match x with
+    | L => simp; exact (sub.apply L  (by simpa using i))
+    | R => simp; exact (sub.apply R  (by simpa using i))
+--    | Tm => simp; exact(sub.apply Tm  (by simpa using i))
+    ⟩
 
 
 @[simp]
-def label.subst (l : label s) (sub : s.subst s') : label s' :=
+def label.subst (l : label s) (sub : LabelSubst s s') : label s' :=
   match l with
-  | .var_label _ s0 => sub.substLbl s0
+  | .var_label _ s0 => sub.apply L s0
   | .latl s0 => .latl s0
   | .ljoin s0 s1 =>
       let s0' := s0.subst sub
@@ -671,10 +729,9 @@ def label.subst (l : label s) (sub : s.subst s') : label s' :=
       let s0' := s0.subst sub
       let s1' := s1.subst sub
       .lmeet s0' s1'
-  | .default => .default
 
 @[simp]
-def corruption.subst (c : corruption s) (sub : s.subst s') : corruption s' :=
+def corruption.subst (c : corruption s) (sub : LabelSubst s s') : corruption s' :=
   match c with
   | .corr l1 =>
       let l1' := l1.subst sub
@@ -684,7 +741,7 @@ def corruption.subst (c : corruption s) (sub : s.subst s') : corruption s' :=
       .not_corr l1'
 
 @[simp]
-def constr.subst (c : constr s) (sub : s.subst s') : constr s' :=
+def constr.subst (c : constr s) (sub : LabelSubst s s') : constr s' :=
   match c with
   | .condition s0 s1 s2 =>
       let s1' := s1.subst sub
@@ -692,59 +749,100 @@ def constr.subst (c : constr s) (sub : s.subst s') : constr s' :=
       .condition s0 s1' s2'
 
 
-def rexp.subst (r : rexp s) (sub : s.subst s') : rexp s' :=
+def rexp.subst (r : rexp s) (sub : RexpSubst s s') : rexp s' :=
   match r with
-  | .fvar i => .fvar i
-  | .var j => sub.substRef j
+  | .fvar nm => .fvar nm
+  | .var j => sub.apply R j
   | .op s r1 r2 =>
       let r1' := r1.subst sub
       let r2' := r2.subst sub
       .op s r1' r2'
   | .const b => .const b
-  | .tmvar j => sub.substTm j
 
-def prop.subst (p : prop s) (sub : s.subst s') : prop s' :=
+def prop.subst (p : prop s) (sub : RexpSubst s s') : prop s' :=
   match p with
   | .peq re1 re2 => .peq (re1.subst sub) (re2.subst sub)
   | .pand p1 p2 => .pand (p1.subst sub) (p2.subst sub)
   | .por p1 p2 => .por (p1.subst sub) (p2.subst sub)
   | .pimpl p1 p2 => .pimpl (p1.subst sub) (p2.subst sub)
   | .pnot p1 => .pnot (p1.subst sub)
-  | .pall p => .pall (p.subst sub.bumpRef)
+  | .pall p => .pall (p.subst $ sub.bump R)
 
 
 @[simp]
-def ty.subst (t : ty s) (sub : s.subst s') : ty s' :=
+def ty.subst (t : ty s) (sub : Subst s s') : ty s' :=
   match t with
   | .admit => .admit
-  | .var_ty s0 => sub.substTy s0
+  | .var_ty s0 => sub.apply Ty s0
   | .Any => .Any
   | .Unit => .Unit
-  | .RData s0 re => .RData (s0.subst sub) (re.subst sub)
-  | .Data s0 => .Data (s0.subst sub)
+  | .RData s0 re => .RData (s0.subst sub.toLabelSubst) (re.subst sub.toRexpSubst)
+  | .Data s0 => .Data (s0.subst sub.toLabelSubst)
   | .Ref s0 => .Ref (s0.subst sub)
-  | .refined t p => .refined (t.subst sub) (p.subst sub)
+  | .refined t p => .refined (t.subst sub) (p.subst sub.toRexpSubst)
   | .arr s0 s1 => .arr (s0.subst sub) (s1.subst sub)
   | .union s0 s1 => .union (s0.subst sub) (s1.subst sub)
   | .inter s0 s1 => .inter (s0.subst sub) (s1.subst sub)
   | .prod s0 s1 => .prod (s0.subst sub) (s1.subst sub)
   | .sum s0 s1 => .sum (s0.subst sub) (s1.subst sub)
   | .all s0 s1 =>
-      .all (s0.subst sub) (s1.subst sub.bumpTy)
+      .all (s0.subst sub) (s1.subst $ sub.bump _)
   | .ex s0 s1 =>
-      .ex (s0.subst sub) (s1.subst sub.bumpTy)
+      .ex (s0.subst sub) (s1.subst $ sub.bump _)
   | .ex_r t0 =>
-      .ex_r (t0.subst sub.bumpRef)
+      .ex_r (t0.subst $ sub.bump _)
   | .all_r t0 =>
-      .all_r (t0.subst sub.bumpRef)
+      .all_r (t0.subst $ sub.bump _)
   | .all_l s0 s1 s2 =>
-      .all_l s0 (s1.subst sub) (s2.subst sub.bumpLbl)
+      .all_l s0 (s1.subst sub.toLabelSubst) (s2.subst $ sub.bump _)
   | .t_if s0 s1 s2 =>
-      .t_if (s0.subst sub) (s1.subst sub) (s2.subst sub)
+      .t_if (s0.subst sub.toLabelSubst) (s1.subst sub) (s2.subst sub)
   | .Public => .Public
   | .default => .default
 
+def _root_.Fin.down (f : Fin (n + 1)) : Option (Fin n) :=
+  if h : f < n then .some ⟨f.val, by grind⟩ else none
 
+
+-- Down-coercions
+
+/-
+
+class Down (s t : Type) where
+  down : s -> t
+
+def label.downTy (l : label s.bumpTy) : label s :=
+  match l with
+  | .var_label s0 i => .var_label s0 i
+  | .latl x => .latl x
+  | .ljoin l1 l2 => .ljoin (l1.downTy) (l2.downTy)
+  | .lmeet l1 l2 => .lmeet (l1.downTy) (l2.downTy)
+  | .default => .default
+
+instance : Down (label s.bumpTy) (label s) where
+  down := label.downTy
+
+instance [Down s t] : Down (List s) (List t) where
+  down := fun l => l.map (Down.down ·)
+
+def rexp.downTy (r : rexp s.bumpTy) : rexp s :=
+  match r with
+  | .fvar i => .fvar i
+  | .var j => .var j
+  | .op s r1 r2 => .op s (r1.downTy) (r2.downTy)
+  | .const b => .const b
+  | .tmvar j => .tmvar j
+
+instance : Down (rexp s.bumpTy) (rexp s) where
+  down := rexp.downTy
+
+def label.downTm (l : label s.bumpTm) : label s :=
+  match l with
+  | .var_label s0 i => .var_label s0 i
+  | .latl x => .latl x
+  | .ljoin l1 l2 => .ljoin (l1.downTm) (l2.downTm)
+  | .lmeet l1 l2 => .lmeet (l1.downTm) (l2.downTm)
+  | .default => .default
 
 /-
 
@@ -755,5 +853,6 @@ inductive Decl : ScopeEnv -> ScopeEnv -> Type where
   | DeclApp : Decl se se' -> Decl se' se'' -> Decl se se''
 -/
 
+-/
 
 end Owl
